compiler/src/compilerExamples/swap.v
@@ -62,7 +62,7 @@ Instance pipeline_assumptions: @Pipeline.assumptions pipeline_params. Admitted.
 
 Definition allFuns: list swap.bedrock_func := [swap; swap_swap].
 
-Definition e := RegRename.map.putmany_of_pairs map.empty allFuns.
+Definition e := map.putmany_of_list allFuns map.empty.
 
 Definition main: @cmd.cmd (FlattenExpr.mk_Syntax_params _) :=
   @cmd.call (FlattenExpr.mk_Syntax_params _) [] "swap_swap" [expr.literal 100; expr.literal 108].
